ifc/extended/Testing/Reachability.v
@@ -1,9 +1,7 @@
-Require Import Machine.
+Require Import List. Import ListNotations.
+Require Import ZArith.
 
 Require Import Common.
-
-Require Import List.
-Require Import ZArith.
 
 Definition is_low_pointer (obs : Label) (st : State) (a : Atom) : bool :=
   match a with
@@ -84,8 +82,7 @@ Function reachable_from_root_set (obs : Label) (st : State)
         end
   end.
 Proof.
-admit. admit. admit.
-Defined.
+Admitted.
 
 Definition reachable (obs : Label) (st : State) : list mframe :=
   let root_set := get_root_set obs st in
@@ -98,9 +95,8 @@ Definition well_formed_label (st : State) (l : Label) : bool :=
 (* Given a state and a stamp configuration, make sure everything is ok *)
 (* LL: This also suggests a way of generating stamps! Namely, get
    the meet of all the labels where a frame is reachable *)
-Definition well_formed (top_prin : Label) (st : State) : bool :=
-  let all_labels := map lab_of_list (powerset (Zset.elements top_prin)) in
-  forallb (well_formed_label st) all_labels.
+Definition well_formed (st : State) : bool :=
+  forallb (well_formed_label st) elems.
 
 (* Computes the meet of a list of labels. Must be provided with top as the
    initial accumulator *)
@@ -109,11 +105,9 @@ Definition list_meet (acc : Label) (ls : list Label) :=
 
 (* Attempt to reverse the above predicate to get a stamp generator *)
 (* CH: currently unused *)
-Definition generate_stamp (top_prin : Label) (st : State) (mf : mframe) : mframe :=
-  let all_labels := map lab_of_list (powerset (Zset.elements top_prin)) in
-  let cands := filter (fun l => elem Mem.EqDec_block mf (reachable l st))
-                      all_labels in
-  Mem.put_stamp (list_meet top_prin cands) mf.
+Definition generate_stamp (st : State) (mf : mframe) : mframe :=
+  let cands := filter (fun l => elem Mem.EqDec_block mf (reachable l st)) elems in
+  Mem.put_stamp (list_meet top cands) mf.
 
 
 (* LL: TODO: go through the whole thing and generate stamps! *)
