ifc/extended/Testing/SingleStateArb.v
@@ -24,16 +24,12 @@ Instance arbState : Arbitrary State :=
 {|
   arbitrary := @genState ;
   shrink x :=
-    let '(St _ _ prins _ _ _) := x in
-    let all := shrinkVState (Var prins x x) in
+    let all := shrinkVState (Var top x x) in
     let state_of_var v := let '(Var _ x _) := v in x in
-    filter (indist prins x) (map state_of_var all)
+    filter (indist top x) (map state_of_var all)
 |}.
 
 Instance showState : Show State :=
 {|
-  show x :=
-    let '(St _ _ p _ _ _) := x in
-    show_pair p x x
+  show x := show_pair top x x
 |}.
-
